seiostar/QTypes.fst
@@ -191,8 +191,7 @@ let q_io_res (o:io_ops) : qType =
   | OClose -> qResexn qUnit
 
 let lem_q_io_args (o:io_ops) :
-  Lemma (get_Type (q_io_args o) == io_args o)
-  [SMTPat (q_io_args o)] =
+  Lemma (get_Type (q_io_args o) == io_args o) =
   match o with
   | OOpen -> assert (get_Type (q_io_args OOpen) == io_args OOpen) by (FStar.Tactics.V1.compute (); FStar.Tactics.V1.trefl ())
   | ORead -> assert (get_Type (q_io_args ORead) == io_args ORead) by (FStar.Tactics.V1.compute (); FStar.Tactics.V1.trefl ())
@@ -200,8 +199,7 @@ let lem_q_io_args (o:io_ops) :
   | OClose -> assert (get_Type (q_io_args OClose) == io_args OClose) by (FStar.Tactics.V1.compute (); FStar.Tactics.V1.trefl ())
 
 let lem_q_io_res (o:io_ops) :
-  Lemma (forall (a:io_args o). get_Type (q_io_res o) == io_res o a)
-  [SMTPat (q_io_res o)] =
+  Lemma (forall (a:io_args o). get_Type (q_io_res o) == io_res o a) =
   match o with
   | OOpen -> assert (get_Type (q_io_res OOpen) == resexn file_descr) by (FStar.Tactics.V1.compute (); FStar.Tactics.V1.trefl ())
   | ORead -> assert (get_Type (q_io_res ORead) == resexn string) by (FStar.Tactics.V1.compute (); FStar.Tactics.V1.trefl ())
